kruskal/env_kruskal_edgelist.v
@@ -14,6 +14,8 @@ Definition wedgerep := reptype t_struct_edge.
 Instance wedgerep_inhabitant : Inhabitant wedgerep :=
                                     (Vundef, (Vundef, Vundef)).
 
+Definition t_subset := Tstruct _subset noattr.
+
 
 (*Warning: reptype of a struct doesn’t destruct nicely*)
 Definition def_wedgerep (x: reptype t_struct_edge) :=
